\text{Dadas as funções $f\left( x \right) = 3x - 1$ e $g\left( x \right) = x^{2} + x - 1$, determine: gog\left( x \right)} \\ \\

\text{$\bbox[orange, 8px]{f\left( x \right) = 3x - 1}$ e $\bbox[orange, 8px]{g\left( x \right) = x^{2} + x - 1}$} \\ \\

gog\left( x \right) = g\left( g\left( x \right) \right) = g\left( x^{2} + x - 1  \right) = \left( x^{2} + x - 1\right)^{2} + \left( x^{2} + x - 1 \right) - 1  \\ \\

\text{Cálculo de $\bbox[orange, 8px]{\left( x^{2} + x - 1 \right)^{2}}$ } \\ \\

\left[ x^{2} + \left( x - 1 \right) \right]^{2} = \\ \\

\Rightarrow x^{4} + x^{2} \cdot \left( x - 1 \right) + \left( x - 1 \right)^{2}   \\ \\ 

\Rightarrow x^{4} + 2x^{3}  - 2x^{2} + x^{2} - 2x  + 1 \\ \\ 

\left[ x^{2} + \left( x - 1 \right) \right]^{2} = x^{4} + 2x^{3}  - x^{2} - 2x  + 1 \\ \\ 

\text{Logo: } \\ \\ 

gog\left( x \right) = x^{4} + 2x^{3} -2x - 1 + x^{2} + x - 1 - 1 \\ \\

